not typed BDD

BDD.fst
@@ -1,138 +1,281 @@
 module BDD
 
-open FStar.List
-module S = FStar.Set
-module M = FStar.Map 
+open Compare 
+module M = MapAVL
+module S = SetAVL 
 
 (** type of typed bdd and it's tag for memoization *)
 type bdd': eqtype = {tag: nat; node: node'}
 
-(** sign of the bdd *)
-and sign: eqtype = | INVERSE | IDENTITY
-
 (** a node can be a leaf with it's sign or a node of the form
 sign (low <- var -> high) = (sign low <- var -> sign high) *)
 and node': eqtype = 
-    | Leaf: sign -> node'
-    | Node: sign -> bdd' -> nat -> bdd' -> node'
+    | One:  node'
+    | Zero: node'
+    | Node: bdd' -> nat -> bdd' -> node'
 
 (** give the low bdd of a given bdd *)
 let get_low (bdd: bdd'{Node? bdd.node}) = match bdd.node with 
-    | Node s l v h -> l
+    | Node l v h -> l
 
 (** give the low bdd of a given bdd *)
 let get_high (bdd: bdd'{Node? bdd.node}) = match bdd.node with 
-    | Node s l v h -> h
+    | Node l v h -> h
 
 (** give the low bdd of a given bdd *)
 let get_var (bdd: bdd'{Node? bdd.node}) = match bdd.node with 
-    | Node s l v h -> v
+    | Node l v h -> v
 
-(** give the low bdd of a given bdd *)
-let get_sign (bdd: bdd'{Node? bdd.node}) = match bdd.node with
-    | Node s l v h -> s
-    | Leaf s -> s
+let is_leaf (n: node') : bool = match n with 
+    | Zero | One -> true 
+    | Node _ _ _ -> false 
 
 (** one of the conditions that solve all valid bdd *)
 let rec is_obdd (node:node') : prop = 
     match node with
-    | Leaf s -> true 
-    | Node s l v h -> 
-        (Leaf? l.node || get_var l < v) /\ 
-        (Leaf? h.node || get_var h < v) /\ 
+    | Zero | One -> true 
+    | Node l v h -> l =!= h /\ 
+        (is_leaf l.node || get_var l < v) /\ 
+        (is_leaf h.node || get_var h < v) /\ 
         is_obdd l.node /\ is_obdd h.node
 
-(** more safety type for bdd *)
+(** type for a valid bdd *)
 type bdd  = bdd:bdd'  {is_obdd bdd.node}
+
+(** type for a valid node *)
 type node = node:node'{is_obdd node}
 
-(** allow to compare bdd without deep comparaison *)
-type hash_type = bool & bool & nat & nat & nat
-private let node_hash (node:node) : hash_type = 
-    match node with 
-    | Node INVERSE l v h  -> true, true,  l.tag, v, h.tag 
-    | Node IDENTITY l v h -> true, false, l.tag, v, h.tag 
-    | Leaf INVERSE  -> false, true,  0, 0, 0
-    | Leaf IDENTITY -> false, false, 0, 0, 0
+let rec eval_node (f: nat -> bool) (node:node') : bool
+    = match node with 
+    | One  -> true 
+    | Zero -> false 
+    | Node l v h -> 
+        if f v then eval_node f h.node else eval_node f l.node
 
-noeq
-type global_table = {
-    map: M.t hash_type bdd;
-    size: nat
+(** comparaison function for integer *)
+private let compareInt : comparaison int = fun x y -> 
+    if x > y then GT else if x < y then LT else EQ 
+
+(** comparaison function for node *)
+let compareNode : comparaison node = fun (l:node) (h:node) ->
+    match l, h with
+    | Node ll lv lh, Node hl hv hh ->  
+    begin
+        match compareInt ll.tag hl.tag with 
+        | EQ -> begin match compareInt lh.tag hh.tag with 
+            | EQ ->  compareInt lv hv 
+            | x -> x end 
+        | x -> x
+    end 
+    | Zero, Node _ _ _ -> GT 
+    | One , Node _ _ _ -> GT 
+    | Node _ _ _, Zero -> LT 
+    | Node _ _ _, One  -> LT 
+    | Zero, One -> LT 
+    | One, Zero -> GT 
+    | _, _ -> EQ 
+
+(** a table of node/bdd and it's cardinal *)
+type global_table' = {
+    map: M.map node bdd compareNode; 
+    size: nat;
 }
 
-let is_correct_table (table:global_table) : prop = 
-    forall hash. M.contains table.map hash ==> (
-        let bdd = M.sel table.map hash in 
+(** a good memoization table !!! *)
+let is_valid_table (table:global_table') : prop = 
+    M.member (One)  ({tag=1; node=One }) table.map /\
+    M.member (Zero) ({tag=0; node=Zero}) table.map /\
+    (forall (node:node) (bdd:bdd). M.member node bdd table.map ==> (
 
-        (* on veut pouvoir en conclure une relation du type
-            bdd == (M.sel table.map (node_hash bdd.node))  *)
-        node_hash bdd.node == hash /\ 
-
-        (* pour la génération de futur bdd *)
+        (* each pair bdd node is valid *)
+        bdd.node == node /\
+        
+        (* ==> easy to create a new tag *)
         bdd.tag < table.size /\ 
 
-        (* unicité des bdd dans la table à leurs tag près *)
-        (forall hash'. 
-            M.contains table.map hash' ==> (
-            let bdd' = M.sel table.map hash' in 
-            (bdd'.tag = bdd.tag ==> bdd' == bdd) /\ 
-            (bdd'.node == bdd.node ==> bdd' == bdd)
+        (* unicity of tag *)
+        (forall n b. M.member n b table.map ==> (
+            bdd.tag == b.tag ==> bdd == b
         )) /\
 
-        (* les fils d'un noeud doivent être dans la table *)
-        begin match bdd.node with 
-        | Node s l v h -> 
-            M.contains table.map (node_hash l.node) /\ 
-            M.contains table.map (node_hash h.node) /\ 
-            M.sel table.map (node_hash l.node) == l /\
-            M.sel table.map (node_hash h.node) == h
-        | Leaf s -> true 
-        end 
-    )
+        (* recursivity property *)
+        (is_leaf node \/ (
+            let l = get_low  bdd in 
+            let h = get_high bdd in 
+            M.member l.node l table.map /\ 
+            M.member h.node h table.map
+        ))
+    ))
 
-type valid_table = table:global_table{is_correct_table table}
+(** type of valid table *)
+type global_table = table:global_table'{is_valid_table table}
 
-let contains_prop (table:valid_table) (bdd:bdd) : prop = 
-    M.contains table.map (node_hash bdd.node) /\ (M.sel table.map (node_hash bdd.node)) == bdd
 
-let is_compatible_node (table:valid_table) (node:node) : prop = 
+let measure (node:node') : nat = match node with 
+    | Zero | One -> 0 | Node _ v _ -> v + 1
+
+let compatible_node (table:global_table) (node:node): prop = 
     match node with 
-    | Leaf s -> true 
-    | Node s l v h -> 
-        contains_prop table l /\ contains_prop table h
+    | Zero | One -> true 
+    | Node l v h -> 
+        M.member l.node l table.map /\ 
+        M.member h.node h table.map
 
-let rec contains_lemma1 (table:valid_table) (node:node) : 
+#push-options "--z3rlimit 50"
+let contain_lemma1 (table:global_table) (node:node) : 
     Lemma 
-        (requires M.contains table.map (node_hash node))
+        (requires compatible_node table node) 
 
-        (ensures (contains_prop table (M.sel table.map (node_hash node))))
-
-        (decreases (match node with | Node s l v r -> v+1 | Leaf s -> 0))
-    = 
-
-    let bdd = M.sel table.map (node_hash node) in 
-    match bdd.node with 
-    | Leaf s -> ()
-    | Node s l v h -> 
-        assert (Leaf? l.node || get_var l < v);
-        assert (Leaf? l.node || get_var l < v);
-        contains_lemma1 table l.node;
-        contains_lemma1 table h.node
-
-let contains_lemma2 (table:valid_table) (hash:hash_type) : 
-    Lemma 
-        (requires M.contains table.map hash)
-
-        (ensures (contains_prop table (M.sel table.map hash)))
-
-    = let bdd = M.sel table.map hash in 
+        (ensures (
+            match M.find node table.map with
+            | Some (n, b) -> n == node /\ b.node == node
+            | None -> true
+        ))
     
-    assert (node_hash bdd.node == hash);
-    assert (M.contains table.map (node_hash bdd.node));
-    assert (M.sel table.map (node_hash bdd.node) == bdd);
-    contains_lemma1 table bdd.node
+    = match M.find node table.map with
+    | None -> ()
 
-let inv (sign:sign) = match sign with 
-    | INVERSE -> IDENTITY
-    | IDENTITY -> INVERSE
+    | Some (n, b) ->
+    begin
+        assert (EQ? (compareNode n node));
+
+        match node with
+        | Zero | One -> ()
+        | Node l v h -> begin
+            assert (M.member l.node l table.map);
+            assert (M.member h.node h table.map);
+            assert (Node? n); 
+
+            assert ((get_low  b).tag == l.tag);
+            assert ((get_high b).tag == h.tag);
+
+            assert (get_var b == v)
+        end
+    end
+#pop-options
+
+
+let contain_lemma2 (table:global_table) (node:node) :
+    Lemma
+        (requires compatible_node table node)
+
+        (ensures (
+            M.mem node table.map <==> M.member_key node table.map
+        ))
+    
+    = contain_lemma1 table node
+
+#push-options "--z3rlimit 50"
+let makeNode (table: global_table) (node:node') : 
+    Pure
+        (bdd&global_table)
+
+        (requires (
+            match node with 
+            | Zero | One -> true 
+            | Node l v h -> 
+                is_obdd l.node /\ 
+                is_obdd h.node /\
+                M.member l.node l table.map /\
+                M.member h.node h table.map /\
+                (is_leaf l.node || get_var l < v) /\
+                (is_leaf h.node || get_var h < v)
+        ))
+
+        (ensures fun out -> (
+            let bdd, table' = out in 
+            M.member bdd.node bdd table'.map /\ // (Leaf? l.node || get_var l < v) /\
+            (forall n b. M.member n b table.map ==> M.member n b table'.map) /\ 
+            (forall f. eval_node f bdd.node == eval_node f node) /\ 
+            (measure node >= measure bdd.node)
+        ))
+    
+    = match node with 
+    | One  -> ({tag=1; node=node}, table)
+    | Zero -> ({tag=0; node=node}, table)
+    | Node l v h -> 
+    begin 
+        if l.tag = h.tag then (l, table) else 
+        begin 
+            assert (is_obdd node);
+
+            match M.find node table.map with 
+            | Some (n, b) -> 
+            begin 
+                contain_lemma1 table node; 
+                (b, table)
+            end 
+            | None -> 
+            begin 
+                let bdd = {tag=table.size; node=node} in 
+                let table' = {map=M.add table.map node bdd; size=table.size+1} in
+                (bdd, table') 
+            end 
+        end 
+    end 
+
+
+let rec notBDD (table:global_table) (input:bdd) : 
+    Pure 
+        (bdd&global_table)
+
+        (requires M.member input.node input table.map) 
+
+        (ensures fun out -> (
+            let bdd', table' = out in 
+            M.member bdd'.node bdd' table'.map /\ 
+            (forall f. eval_node f bdd'.node == not (eval_node f input.node)) /\ 
+            (forall n b. M.member n b table.map ==> M.member n b table'.map) /\ 
+            (measure input.node >= measure bdd'.node)
+        ))
+
+        (decreases (measure input.node))
+    
+    = match input.node with 
+    | One -> makeNode table Zero
+    | Zero -> makeNode table One
+    | Node l v h -> 
+    begin 
+        let (l', table1) = notBDD table  l in
+        let (h', table2) = notBDD table1 h in 
+        assert (is_obdd l'.node); assert (is_obdd h'.node); 
+        assert (M.member l'.node l' table2.map); 
+        assert (M.member h'.node h' table2.map);
+
+        makeNode table2 (Node l' v h')
+        
+    end 
+#pop-options 
+
+let apply (table: global_table) (f : bool -> bool -> bool) (l: bdd) (r : bdd) : 
+    Pure 
+        (bdd&global_table)
+
+        (requires 
+            M.member l.node l table.map /\ 
+            M.member r.node r table.map 
+        )
+
+        (ensures fun out -> (
+            let bdd', table' = out in 
+            M.member bdd'.node bdd' table'.map /\ 
+            (forall n b. M.member n b table.map ==> M.member n b table'.map) /\ 
+            (forall g. eval_node g bdd'.node == f (eval_node g l.node) (eval_node g r.node))
+        ))
+    
+    = admit ()
+
+let restrict (table:global_table) (n:nat) (b:bool) (input:bdd) : 
+    Pure 
+        (bdd&global_table)
+
+        (requires M.member input.node input table.map)
+
+        (ensures fun out -> (
+            let bdd', table' = out in 
+            M.member bdd'.node bdd' table'.map /\ 
+            (forall n b. M.member n b table.map ==> M.member n b table'.map) /\ 
+            (forall f. eval_node f bdd'.node == eval_node (fun i -> if i = n then b else f i) input.node)
+        ))
+    
+    = admit ()
